mk_read_repr_impl

examples/layeredeffects/LowParseWriters.fst
@@ -39,6 +39,11 @@ let read_repr_impl
     res == spec ()
   ))
 
+let mk_read_repr_impl
+  a pre post post_err l spec impl
+=
+  impl
+
 let read_return_impl
   a x inv
 = fun _ -> Correct x
